codeTest/CorrectRel.v
@@ -1,6 +1,6 @@
 From dx.tests Require Import DxIntegers DxValues DxMemRegion DxRegs DxState DxMonad DxInstructions.
 From Coq Require Import List Lia.
-From compcert Require Import Integers Values Clight Memory.
+From compcert Require Import Integers Values Clight Memory AST.
 Import ListNotations.
 Require Import ZArith.
 
@@ -16,3 +16,14 @@ Definition val64_correct (x:val64_t) (v: val) :=
 Definition reg_correct (r: reg) (v: val) (stm:stateM) (m: Memory.Mem.mem) :=
   (*complu_lt_32 v (Vint (Int.repr 11)) = true /\ (**r ensured by verifier *) *)
     v = Vint (Int.repr (id_of_reg r)).
+
+
+Definition match_chunk (x : memory_chunk) (b: val) :=
+  b = Vint (
+          match x with
+          | Mint8unsigned => Integers.Int.one
+          | Mint16unsigned => Integers.Int.repr 2
+          | Mint32 => Integers.Int.repr 4
+          | Mint64 => Integers.Int.repr 8
+          | _ => Integers.Int.repr 0
+          end).
